Made the InitLibrary operation abstract

tutorial/utp_library.thy
@@ -24,19 +24,15 @@ alphabet library =
   books :: "book set"
   loans :: "book set"
 
-abbreviation "Books \<equiv> {''War and Peace''
-                       ,''Pride and Prejudice''
-                       ,''Les Miserables''}"
-
 subsection {* Library operations *}
   
-definition InitLibrary :: "library prog" where
-[upred_defs]: "InitLibrary = true \<turnstile>\<^sub>n books, loans := \<guillemotleft>Books\<guillemotright>, {}\<^sub>u"
+definition InitLibrary :: "book set \<Rightarrow> library prog" where
+[upred_defs]: "InitLibrary(bs) = true \<turnstile>\<^sub>n books, loans := \<guillemotleft>bs\<guillemotright>, {}\<^sub>u"
   
-definition InitLibraryAlt :: "library prog" where
-[upred_defs]: "InitLibraryAlt = true \<turnstile>\<^sub>n ($books\<acute> =\<^sub>u \<guillemotleft>Books\<guillemotright> \<and> $loans\<acute> =\<^sub>u {}\<^sub>u)"
+definition InitLibraryAlt :: "book set \<Rightarrow> library prog" where
+[upred_defs]: "InitLibraryAlt(bs) = true \<turnstile>\<^sub>n ($books\<acute> =\<^sub>u \<guillemotleft>bs\<guillemotright> \<and> $loans\<acute> =\<^sub>u {}\<^sub>u)"
 
-lemma InitLibrary_alt_same: "InitLibrary = InitLibraryAlt"
+lemma InitLibrary_alt_same: "InitLibrary(bs) = InitLibraryAlt(bs)"
   by (rel_auto)
 
 definition LibraryInvariant :: "library upred" where
@@ -50,7 +46,7 @@ definition ReturnBook :: "book \<Rightarrow> library prog" where
 
 subsection {* Library proofs *}
 
-lemma InitLibrary_Idempotent: "InitLibrary ;; InitLibrary = InitLibrary"
+lemma InitLibrary_Idempotent: "InitLibrary(bs) ;; InitLibrary(bs) = InitLibrary(bs)"
   by (rel_blast)
 
 lemma BorrowBook_Twice: "(BorrowBook(b) ;; BorrowBook(b)) = abort"
@@ -59,32 +55,20 @@ lemma BorrowBook_Twice: "(BorrowBook(b) ;; BorrowBook(b)) = abort"
 lemma ReturnBook_Twice: "(ReturnBook(b) ;; ReturnBook(b)) = abort"
   by (rel_auto)
 
+abbreviation "Books \<equiv> {''War and Peace''
+                       ,''Pride and Prejudice''
+                       ,''Les Miserables''}"
+    
 lemma NotInLibrary:
-  "(InitLibrary ;; BorrowBook(''Pride and Prejudice and Zombies'')) = abort"
+  "(InitLibrary(Books) ;; BorrowBook(''Pride and Prejudice and Zombies'')) = abort"
   by (rel_auto)
 
-text {*
-  Simon, originally this proof went through with @{text "(rel_blast)"} alone
-  but it took a lot of time (15 secs). I revised it to go through faster...
-  In the future, I think it is good practice \emph{not} to leave proofs that
-  take such a long time in the scripts as this causes a long delays when we
-  building the system to validate merges, and we frequently have to do this.
-  If you know the proof goes through, perhaps comment out the script as TODO
-  and add the lemma as a sorry before committing to Github. Cheers, Frank.
-*}
-
 theorem BorrowAndReturn: 
-  assumes "b \<in> Books"
-  shows "(InitLibrary ;; BorrowBook(b) ;; ReturnBook(b)) = InitLibrary"
-  using assms
-  apply (rel_simp)
--- {* Give blast a little help... *}
-  apply (case_tac "ok\<^sub>v")
-  apply (simp_all)
-  apply (blast)+
-done
+  assumes "b \<in> bs"
+  shows "(InitLibrary(bs) ;; BorrowBook(b) ;; ReturnBook(b)) = InitLibrary(bs)"
+  using assms by (rel_blast)
 
-lemma "InitLibrary establishes LibraryInvariant"
+lemma "InitLibrary(bs) establishes LibraryInvariant"
   by (rel_auto)
 
 lemma "BorrowBook(b) maintains LibraryInvariant"
@@ -92,4 +76,5 @@ lemma "BorrowBook(b) maintains LibraryInvariant"
     
 lemma "ReturnBook(b) maintains LibraryInvariant"
   by (rel_auto)
+
 end
